feat: cleaned up add chip

SP1Operations/AddOperation.lean
@@ -2,16 +2,9 @@ import SP1Foundations
 
 namespace AddOperation
 
-def spec
-  (a0 a1 : U16)
-  (b0 b1 : U16)
-  (c0 c1 : U16)
-  (is_real : U1) : Prop :=
-    is_real = 1 → BitVec.ofU16 a0 a1 = BitVec.ofU16 b0 b1 + BitVec.ofU16 c0 c1
-
 def constraints
   (I : Vector BabyBear 7)
-  : List SP1Constraint :=
+  : SP1ConstraintList :=
   let E0 := I[6] - 1
   let E2 := I[6] * E0
   let E4 := I[0] + I[2]
@@ -35,9 +28,16 @@ def constraints
   , .send (.byte (ByteOpcode.ofNat 6) I[5] 16 0) I[6]
   ]
 
-def constraints'
-  (I : Vector BabyBear 7)
-  : Prop :=
+-- Should we be including the bounds at this level? Instead done below seperately
+def spec
+  (a0 a1 : U16)
+  (b0 b1 : U16)
+  (c0 c1 : U16)
+  (is_real : U1) : Prop :=
+    is_real = 1 → BitVec.ofU16 a0 a1 = BitVec.ofU16 b0 b1 + BitVec.ofU16 c0 c1
+
+def constraintsProp
+  (I : Vector BabyBear 7) : Prop :=
   let carry0  : BabyBear := 0
   let carry1  : BabyBear := (I[0] + I[2] - I[4] + carry0) * (baseInv : BabyBear)
   let carry2  : BabyBear := (I[1] + I[3] - I[5] + carry1) * (baseInv : BabyBear)
@@ -49,20 +49,19 @@ def constraints'
     (I[5] < 65536)
   )
 
-def constraints_iff_constraints'
-  (I : Vector BabyBear 7)
-  : List.Forall SP1Constraint.toProp (constraints I) ↔ constraints' I := by
+def constraints_iff_constraintsProp
+  (I : Vector BabyBear 7) : (constraints I).allHold ↔ constraintsProp I := by
   by_cases h : I[6] = 0
-  · simp [constraints, constraints', h]
-  · by_cases h' : I[6] = 1 <;> simp [constraints, constraints', h, h', sub_eq_zero]
+  · simp [constraints, constraintsProp, h]
+  · by_cases h' : I[6] = 1 <;> simp [constraints, constraintsProp, h, h', sub_eq_zero]
 
 theorem correct
   (a0 a1 b0 b1 c0 c1 : U16)
   (is_real : U1) :
-    List.Forall SP1Constraint.toProp (constraints #v[b0, b1, c0, c1, a0, a1, is_real]) →
+    (constraints #v[b0, b1, c0, c1, a0, a1, is_real]).allHold →
     spec a0 a1 b0 b1 c0 c1 is_real := by
-  rw [constraints_iff_constraints' (#v[b0, b1, c0, c1, a0, a1, is_real])]
-  simp [constraints', spec]
+  rw [constraints_iff_constraintsProp (#v[b0, b1, c0, c1, a0, a1, is_real])]
+  simp [constraintsProp, spec]
   intro q1
 
   intro h_is_real
@@ -84,5 +83,35 @@ theorem correct
       simp [Fin.mul_def, Fin.sub_def, Fin.add_def, Fin.ext_iff, BabyBearPrime] at *
       rw [Fin.lt_def] at qq3 aa4
       aesop (add 50% tactic (by omega))
+
+open BitVec
+
+lemma lt_of_constraintsAllHold {c0 c1 a0 a1 b0 b1 : BabyBear}
+    (h : (constraints #v[c0, c1, b0, b1, a0, a1, 1]).allHold) : a0 < 65536 := by
+  rw [constraints_iff_constraintsProp] at h
+  rw [constraintsProp] at h
+  simp at h
+  tauto
+
+lemma lt_of_constraintsAllHold' {c0 c1 a0 a1 b0 b1 : BabyBear}
+    (h : (constraints #v[c0, c1, b0, b1, a0, a1, 1]).allHold) : a1 < 65536 := by
+  rw [constraints_iff_constraintsProp] at h
+  rw [constraintsProp] at h
+  simp at h
+  tauto
+
+/-- Version of correctness using specific bitvecs.
+To get good rewrites we allow arbitrary proofs on the left (should do the reverse for ← rw to work)-/
+lemma correct' (c0 c1 : BabyBear) (a0 a1 b0 b1 : U16)
+    (h : (constraints #v[a0, a1, b0, b1, c0, c1, 1]).allHold)
+    (pf : c0.val + c1.val * 65536 < 2 ^ 32) :
+    (c0.val + c1.val * 65536)#'pf =
+      (BitVec.ofU16 a0 a1 + BitVec.ofU16 b0 b1) := by
+  let c0' : U16 := ⟨c0, lt_of_constraintsAllHold h⟩
+  let c1' : U16 := ⟨c1, lt_of_constraintsAllHold' h⟩
+  refine correct c0' c1' a0 a1 b0 b1 1 ?_ rfl
+  exact h
+
+
 
 end AddOperation
